\section{С двумя R}

\paragraph{RXR}

$$R_1XR_2 = 
\begin{pmatrix}
 \frac{{h_x}\sin{\left( {\alpha_2}+{\alpha_1}\right) } }{2}+\frac{{h_x}\sin{\left( {\alpha_2}-{\alpha_1}\right) } }{2}+\cos{\left( {\alpha_2}+{\alpha_1}\right) } & 
 \frac{{h_x}\cos{\left( {\alpha_2}+{\alpha_1}\right) } }{2}+\frac{{h_x}\cos{\left( {\alpha_2}-{\alpha_1}\right) } }{2}-\sin{\left( {\alpha_2}+{\alpha_1}\right) } \\
-\frac{{h_x}\cos{\left( {\alpha_2}+{\alpha_1}\right) } }{2}+\frac{{h_x}\cos{\left( {\alpha_2}-{\alpha_1}\right) } }{2}+\sin{\left( {\alpha_2}+{\alpha_1}\right) } & 
 \frac{{h_x}\sin{\left( {\alpha_2}+{\alpha_1}\right) } }{2}-\frac{{h_x}\sin{\left( {\alpha_2}-{\alpha_1}\right) } }{2}+\cos{\left( {\alpha_2}+{\alpha_1}\right) }
\end{pmatrix}
$$

Обозначим 
$$\alpha_2 - \alpha_1 = \delta;$$
$$\alpha_2 + \alpha_1 = \sigma.$$

$$R_1XR_2 = 
\begin{pmatrix}
 \frac{{h_x}\sin\sigma }{2}+\frac{{h_x}\sin\delta }{2}+\cos\delta & 
 \frac{{h_x}\cos\sigma }{2}+\frac{{h_x}\cos\delta }{2}-\sin\delta \\
-\frac{{h_x}\cos\sigma }{2}+\frac{{h_x}\cos\delta }{2}+\sin\delta & 
 \frac{{h_x}\sin\sigma }{2}-\frac{{h_x}\sin\delta }{2}+\cos\delta
\end{pmatrix}
$$

$$b_{11} - b_{22} = h_x \sin\delta;$$
$$b_{12} + b_{21} = h_x \cos\delta ;$$

$$\left(b_{11} - b_{22}\right)^2 + \left(b_{12} + b_{21}\right)^2 = h_x^2;$$
$$\sin\delta = \frac{b_{11} - b_{22}}{h_x};$$
$$\cos\delta = \frac{b_{12} + b_{21}}{h_x};$$

$$\frac{{h_x}\sin\sigma }{2} + \frac{{h_x}\sin\delta }{2} = b_{11} - \cos\delta;$$
$$\sin\sigma + \sin\delta = \frac{2 (b_{11} - \cos\delta)}{h_x};$$
$$\sin\sigma = \frac{2 (b_{11} - \cos\delta)}{h_x} - \sin\delta;$$

$$\sin\sigma + \sin\delta = 2 \cos\alpha_1 \sin\alpha_2;$$
$$\cos\alpha_1 \sin\alpha_2 = \frac{b_{11} - \cos\delta}{h_x};$$


$$\frac{{h_x}\cos\sigma }{2} + \frac{{h_x}\cos\delta }{2} = b_{12} + \sin\delta;$$
$$\cos\sigma + \cos\delta = \frac{2 (b_{12} + \sin\delta)}{h_x};$$
$$\cos\sigma = \frac{2 (b_{12} + \sin\delta)}{h_x} - \cos\delta;$$

$$\cos\sigma + \cos\delta = 2 \cos\alpha_1 \cos\alpha_2;$$
$$\cos\alpha_1 \cos\alpha_2 = \frac{b_{12} + \sin\delta}{h_x};$$

$$\left( \frac{b_{11} - \cos\delta}{h_x} \right)^2 + \left( \frac{b_{12} + \sin\delta}{h_x} \right)^2 = \cos^2 \alpha_1;$$
$$\frac{\left( b_{11} - \cos\delta \right)^2 + \left(b_{12} + \sin\delta\right)^2}{h_x^2} = \cos^2 \alpha_1;$$

$$\sin\alpha_2 = \frac{b_{11} - \cos\delta}{h_x \cos\alpha_1};$$
$$\cos\alpha_2 = \frac{b_{12} + \sin\delta}{h_x \cos\alpha_1};$$


\paragraph{RYR}

$$R_1YR_2 =
\begin{pmatrix}
-\frac{{h_y} \sin{\left( {\alpha_2}+{\alpha_1}\right) } }{2}+\frac{{h_y} \sin{\left( {\alpha_2}-{\alpha_1}\right) } }{2}+\cos{\left( {\alpha_2}+{\alpha_1}\right) } & 
-\frac{{h_y} \cos{\left( {\alpha_2}+{\alpha_1}\right) } }{2}+\frac{{h_y} \cos{\left( {\alpha_2}-{\alpha_1}\right) } }{2}-\sin{\left( {\alpha_2}+{\alpha_1}\right) }\\
 \frac{{h_y} \cos{\left( {\alpha_2}+{\alpha_1}\right) } }{2}+\frac{{h_y} \cos{\left( {\alpha_2}-{\alpha_1}\right) } }{2}+\sin{\left( {\alpha_2}+{\alpha_1}\right) } & 
-\frac{{h_y} \sin{\left( {\alpha_2}+{\alpha_1}\right) } }{2}-\frac{{h_y} \sin{\left( {\alpha_2}-{\alpha_1}\right) } }{2}+\cos{\left( {\alpha_2}+{\alpha_1}\right) }
\end{pmatrix}
$$

Обозначим 
$$\alpha_2 - \alpha_1 = \delta;$$
$$\alpha_2 + \alpha_1 = \sigma.$$

$$R_1YR_2 =
\begin{pmatrix}
-\frac{{h_y} \sin\sigma }{2}+\frac{{h_y}\sin\delta }{2}+\cos\delta  & 
-\frac{{h_y} \cos\sigma }{2}+\frac{{h_y}\cos\delta }{2}-\sin\delta \\
 \frac{{h_y} \cos\sigma }{2}+\frac{{h_y}\cos\delta }{2}+\sin\delta  & 
-\frac{{h_y} \sin\sigma }{2}-\frac{{h_y}\sin\delta }{2}+\cos\delta 
\end{pmatrix}
$$



$$b_{11} - b_{22} = {h_y}\sin\delta  $$
$$b_{12} + b_{21} = {h_y}\cos\delta  $$

$$\left(b_{11} - b_{22}\right)^2 + \left(b_{12} + b_{21}\right)^2 = h_y^2;$$
$$\sin\delta = \frac{b_{11} - b_{22}}{h_y};$$
$$\cos\delta = \frac{b_{12} + b_{21}}{h_y};$$

$$\frac{{h_y} (-\sin\sigma + \sin\delta)}{2} = b_{11} - \cos\delta;$$
$$(-\sin\sigma + \sin\delta) = \frac{2(b_{11} - \cos\delta)}{h_y};$$
$$-\sin\sigma + \sin\delta = -2\sin\alpha_1 \cos\alpha_2;$$
$$-\sin\alpha_1 \cos\alpha_2 = \frac{(b_{11} - \cos\delta)}{h_y};$$

$$\frac{{h_y} (-\cos\sigma + \cos\delta)}{2} = b_{12} + \sin\delta;$$
$$(-\cos\sigma + \cos\delta) = \frac{2(b_{12} + \sin\delta)}{h_y};$$
$$-\cos\sigma + \cos\delta =  2\sin\alpha_1 \sin\alpha_2;$$
$$ \sin\alpha_1 \sin\alpha_2 = \frac{(b_{12} + \sin\delta)}{h_y};$$

$$
\left( \frac{(b_{11} - \cos\delta)}{h_y} \right)^2
+
\left( \frac{(b_{12} + \sin\delta)}{h_y} \right)^2
= \sin^2 \alpha_1
$$

$$ \sin\alpha_2 = \frac{(b_{12} + \sin\delta)}{h_y \sin\alpha_1};$$
$$-\cos\alpha_2 = \frac{(b_{11} - \cos\delta)}{h_y \sin\alpha_1};$$


\paragraph{RSR}

$$R_1SR_2 = 
\begin{pmatrix}
 {s_x}\cos{\left( {\alpha_1}\right) } \cos{\left( {\alpha_2}\right) } - {s_y}\sin{\left( {\alpha_1}\right) } \sin{\left( {\alpha_2}\right) }  & 
-{s_y}\sin{\left( {\alpha_1}\right) } \cos{\left( {\alpha_2}\right) } - {s_x}\cos{\left( {\alpha_1}\right) } \sin{\left( {\alpha_2}\right) } \\
 {s_y}\cos{\left( {\alpha_1}\right) } \sin{\left( {\alpha_2}\right) } + {s_x}\sin{\left( {\alpha_1}\right) } \cos{\left( {\alpha_2}\right) }  & 
 {s_y}\cos{\left( {\alpha_1}\right) } \cos{\left( {\alpha_2}\right) } - {s_x}\sin{\left( {\alpha_1}\right) } \sin{\left( {\alpha_2}\right) } 
\end{pmatrix}
$$



$$a_{11} - a_{22} = - \left( {s_y}-{s_x}\right) \cos{\left( {\alpha_2}-{\alpha_1}\right) } $$

$$a_{12} + a_{21} = \left( {s_y}-{s_x}\right) \sin{\left( {\alpha_2}-{\alpha_1}\right) } $$

Обозначим 
$$\alpha_2 - \alpha_1 = \delta;$$
$$\alpha_2 + \alpha_1 = \sigma.$$

$$
R_1SR_2 = 
\begin{pmatrix}
 \frac{{s_y} \cos{\sigma}}{2} + \frac{{s_x} \cos{\sigma}}{2} - \frac{\cos{\delta} {s_y}}{2} + \frac{\cos{\delta} {s_x}}{2} &
-\frac{{s_y} \sin{\sigma}}{2} - \frac{{s_x} \sin{\sigma}}{2} + \frac{\sin{\delta} {s_y}}{2} - \frac{\sin{\delta} {s_x}}{2}\\
 \frac{{s_y} \sin{\sigma}}{2} + \frac{{s_x} \sin{\sigma}}{2} + \frac{\sin{\delta} {s_y}}{2} - \frac{\sin{\delta} {s_x}}{2} &
 \frac{{s_y} \cos{\sigma}}{2} + \frac{{s_x} \cos{\sigma}}{2} + \frac{\cos{\delta} {s_y}}{2} - \frac{\cos{\delta} {s_x}}{2}
\end{pmatrix}
$$
$$
R_1SR_2 = 
\begin{pmatrix}
 \frac{(s_y + s_x) \cos{\sigma}}{2} - \frac{(s_y - s_x)\cos{\delta}}{2} &
-\frac{(s_y + s_x) \sin{\sigma}}{2} + \frac{(s_y - s_x)\sin{\delta}}{2}\\
 \frac{(s_y + s_x) \sin{\sigma}}{2} + \frac{(s_y - s_x)\sin{\delta}}{2} &
 \frac{(s_y + s_x) \cos{\sigma}}{2} + \frac{(s_y - s_x)\cos{\delta}}{2}
\end{pmatrix}
$$

$$a_{11} - a_{22} = - \left( {s_y}-{s_x}\right) \cos\delta $$

$$a_{12} + a_{21} = \left( {s_y}-{s_x}\right) \sin\delta $$

$$\left(a_{11} - a_{22}\right)^2 + \left( a_{12} + a_{21} \right)^2 = \left( {s_y}-{s_x}\right)^2.$$

Обозначим
$${s_y}-{s_x} = d_s;$$

$$\left(a_{11} - a_{22}\right)^2 + \left( a_{12} + a_{21} \right)^2 = d_s^2.$$

$$a_{11} - a_{22} = - d_s \cos\delta $$
$$a_{12} + a_{21} = d_s \sin\delta $$

$$\cos\delta = -\frac{a_{11} - a_{22}}{d_s} $$
$$\sin\delta =  \frac{a_{12} + a_{21}}{d_s} $$

$$\begin{cases}
	s_x s_y = \det A,\\
	{s_y} - {s_x} = d_s;
\end{cases}
\Rightarrow
\begin{cases}
	s_x = \frac{1}{2}\left(\pm \sqrt{d_s^2 + 4 \det A} - d_s\right),\\
	s_y = \frac{1}{2}\left(\pm \sqrt{d_s^2 + 4 \det A} + d_s\right).
\end{cases}
$$
Верхние и нижние знаки должны согласованы
	
$$s_x + s_y = \pm \sqrt{d_s^2 + 4 \det A}.$$
	
$$ (s_y + s_x) \cos{\sigma} - (s_y - s_x)\cos{\delta} = 2 a_{11};$$
$$ (s_y + s_x) \cos{\sigma} = 2 a_{11} + (s_y - s_x)\cos{\delta};$$
$$\cos{\sigma} = \frac{2 a_{11}}{(s_y + s_x)} + \frac{(s_y - s_x)}{(s_y + s_x)}\cos{\delta};$$

$$-(s_y + s_x) \sin{\sigma} + (s_y - s_x)\sin{\delta} = 2 a_{12};$$
$$(s_y + s_x) \sin{\sigma} = - 2 a_{12} + (s_y - s_x)\sin{\delta};$$
$$\sin{\sigma} = - \frac{2 a_{12}}{(s_y + s_x)} + \frac{(s_y - s_x)}{(s_y + s_x)}\sin{\delta};$$

$$\sin\sigma = \sin\alpha_1 \cos\alpha_2 + \cos\alpha_1 \sin\alpha_2;$$
$$\cos\sigma = \cos\alpha_1 \cos\alpha_2 - \sin\alpha_1 \sin\alpha_2;$$
$$\sin\delta = - \sin\alpha_1 \cos\alpha_2 + \cos\alpha_1 \sin\alpha_2;$$
$$\cos\delta =\cos\alpha_1 \cos\alpha_2 + \sin\alpha_1 \sin\alpha_2;$$

$$\sin\sigma + \sin\delta = 2\cos\alpha_1 \sin\alpha_2;$$
$$\cos\sigma + \cos\delta = 2\cos\alpha_1 \cos\alpha_2;$$
