\subsection{С двумя R}

\paragraph{RXR}

$$R_1XR_2 = 
\begin{pmatrix}
 \frac{{h_x}\sin{\left( {\alpha_2}+{\alpha_1}\right) } }{2}+\frac{{h_x}\sin{\left( {\alpha_2}-{\alpha_1}\right) } }{2}+\cos{\left( {\alpha_2}+{\alpha_1}\right) } & 
 \frac{{h_x}\cos{\left( {\alpha_2}+{\alpha_1}\right) } }{2}+\frac{{h_x}\cos{\left( {\alpha_2}-{\alpha_1}\right) } }{2}-\sin{\left( {\alpha_2}+{\alpha_1}\right) } \\
-\frac{{h_x}\cos{\left( {\alpha_2}+{\alpha_1}\right) } }{2}+\frac{{h_x}\cos{\left( {\alpha_2}-{\alpha_1}\right) } }{2}+\sin{\left( {\alpha_2}+{\alpha_1}\right) } & 
 \frac{{h_x}\sin{\left( {\alpha_2}+{\alpha_1}\right) } }{2}-\frac{{h_x}\sin{\left( {\alpha_2}-{\alpha_1}\right) } }{2}+\cos{\left( {\alpha_2}+{\alpha_1}\right) }
\end{pmatrix}
$$

Обозначим 
$$\alpha_2 - \alpha_1 = \delta;$$
$$\alpha_2 + \alpha_1 = \sigma.$$

$$R_1XR_2 = 
\begin{pmatrix}
 \frac{{h_x}\sin\sigma }{2}+\frac{{h_x}\sin\delta }{2}+\cos\delta & 
 \frac{{h_x}\cos\sigma }{2}+\frac{{h_x}\cos\delta }{2}-\sin\delta \\
-\frac{{h_x}\cos\sigma }{2}+\frac{{h_x}\cos\delta }{2}+\sin\delta & 
 \frac{{h_x}\sin\sigma }{2}-\frac{{h_x}\sin\delta }{2}+\cos\delta
\end{pmatrix}
$$

$$b_{11} - b_{22} = h_x \sin\delta;$$
$$b_{12} + b_{21} = h_x \cos\delta ;$$

$$\left(b_{11} - b_{22}\right)^2 + \left(b_{12} + b_{21}\right)^2 = h_x^2;$$
$$\sin\delta = \frac{b_{11} - b_{22}}{h_x};$$
$$\cos\delta = \frac{b_{12} + b_{21}}{h_x};$$

$$\frac{{h_x}\sin\sigma }{2} + \frac{{h_x}\sin\delta }{2} = b_{11} - \cos\delta;$$
$$\sin\sigma + \sin\delta = \frac{2 (b_{11} - \cos\delta)}{h_x};$$
$$\sin\sigma = \frac{2 (b_{11} - \cos\delta)}{h_x} - \sin\delta;$$

$$\sin\sigma + \sin\delta = 2 \cos\alpha_1 \sin\alpha_2;$$
$$\cos\alpha_1 \sin\alpha_2 = \frac{b_{11} - \cos\delta}{h_x};$$


$$\frac{{h_x}\cos\sigma }{2} + \frac{{h_x}\cos\delta }{2} = b_{12} + \sin\delta;$$
$$\cos\sigma + \cos\delta = \frac{2 (b_{12} + \sin\delta)}{h_x};$$
$$\cos\sigma = \frac{2 (b_{12} + \sin\delta)}{h_x} - \cos\delta;$$

$$\cos\sigma + \cos\delta = 2 \cos\alpha_1 \cos\alpha_2;$$
$$\cos\alpha_1 \cos\alpha_2 = \frac{b_{12} + \sin\delta}{h_x};$$

$$\left( \frac{b_{11} - \cos\delta}{h_x} \right)^2 + \left( \frac{b_{12} + \sin\delta}{h_x} \right)^2 = \cos^2 \alpha_1;$$
$$\frac{\left( b_{11} - \cos\delta \right)^2 + \left(b_{12} + \sin\delta\right)^2}{h_x^2} = \cos^2 \alpha_1;$$

$$\sin\alpha_2 = \frac{b_{11} - \cos\delta}{h_x \cos\alpha_1};$$
$$\cos\alpha_2 = \frac{b_{12} + \sin\delta}{h_x \cos\alpha_1};$$


\paragraph{RYR}

$$R_1YR_2 =
\begin{pmatrix}
-\frac{{h_y} \sin{\left( {\alpha_2}+{\alpha_1}\right) } }{2}+\frac{{h_y} \sin{\left( {\alpha_2}-{\alpha_1}\right) } }{2}+\cos{\left( {\alpha_2}+{\alpha_1}\right) } & 
-\frac{{h_y} \cos{\left( {\alpha_2}+{\alpha_1}\right) } }{2}+\frac{{h_y} \cos{\left( {\alpha_2}-{\alpha_1}\right) } }{2}-\sin{\left( {\alpha_2}+{\alpha_1}\right) }\\
 \frac{{h_y} \cos{\left( {\alpha_2}+{\alpha_1}\right) } }{2}+\frac{{h_y} \cos{\left( {\alpha_2}-{\alpha_1}\right) } }{2}+\sin{\left( {\alpha_2}+{\alpha_1}\right) } & 
-\frac{{h_y} \sin{\left( {\alpha_2}+{\alpha_1}\right) } }{2}-\frac{{h_y} \sin{\left( {\alpha_2}-{\alpha_1}\right) } }{2}+\cos{\left( {\alpha_2}+{\alpha_1}\right) }
\end{pmatrix}
$$

Обозначим 
$$\alpha_2 - \alpha_1 = \delta;$$
$$\alpha_2 + \alpha_1 = \sigma.$$

$$R_1YR_2 =
\begin{pmatrix}
-\frac{{h_y} \sin\sigma }{2}+\frac{{h_y}\sin\delta }{2}+\cos\delta  & 
-\frac{{h_y} \cos\sigma }{2}+\frac{{h_y}\cos\delta }{2}-\sin\delta \\
 \frac{{h_y} \cos\sigma }{2}+\frac{{h_y}\cos\delta }{2}+\sin\delta  & 
-\frac{{h_y} \sin\sigma }{2}-\frac{{h_y}\sin\delta }{2}+\cos\delta 
\end{pmatrix}
$$



$$b_{11} - b_{22} = {h_y}\sin\delta  $$
$$b_{12} + b_{21} = {h_y}\cos\delta  $$

$$\left(b_{11} - b_{22}\right)^2 + \left(b_{12} + b_{21}\right)^2 = h_y^2;$$
$$\sin\delta = \frac{b_{11} - b_{22}}{h_y};$$
$$\cos\delta = \frac{b_{12} + b_{21}}{h_y};$$

$$\frac{{h_y} (-\sin\sigma + \sin\delta)}{2} = b_{11} - \cos\delta;$$
$$(-\sin\sigma + \sin\delta) = \frac{2(b_{11} - \cos\delta)}{h_y};$$
$$-\sin\sigma + \sin\delta = -2\sin\alpha_1 \cos\alpha_2;$$
$$-\sin\alpha_1 \cos\alpha_2 = \frac{(b_{11} - \cos\delta)}{h_y};$$

$$\frac{{h_y} (-\cos\sigma + \cos\delta)}{2} = b_{12} + \sin\delta;$$
$$(-\cos\sigma + \cos\delta) = \frac{2(b_{12} + \sin\delta)}{h_y};$$
$$-\cos\sigma + \cos\delta =  2\sin\alpha_1 \sin\alpha_2;$$
$$ \sin\alpha_1 \sin\alpha_2 = \frac{(b_{12} + \sin\delta)}{h_y};$$

$$
\left( \frac{(b_{11} - \cos\delta)}{h_y} \right)^2
+
\left( \frac{(b_{12} + \sin\delta)}{h_y} \right)^2
= \sin^2 \alpha_1
$$

$$ \sin\alpha_2 = \frac{(b_{12} + \sin\delta)}{h_y \sin\alpha_1};$$
$$-\cos\alpha_2 = \frac{(b_{11} - \cos\delta)}{h_y \sin\alpha_1};$$
